Just two admits left!

src/x86/procstate.v
@@ -48,18 +48,5 @@ Global Instance ProcStateUpdateOpsDWORD : UpdateOps ProcState PTR DWORD :=
     (ms !p:=b0 !incB p:=b1 !incB(incB p):=b2 !incB(incB(incB p)):=b3).
 
 Definition toSlice (b: BITS 2) := toNat b * 8. 
-
-Definition getRegPiece (v: DWORD) (ix: BITS 2)  := 
-  if ix == #0 then slice 0 8 _ v else
-  if ix == #1 then slice 8 8 _ v else
-  if ix == #2 then slice 16 8 _ v else
-  slice 24 8 _ v.
-
-Definition putRegPiece (v: DWORD) (ix: BITS 2) (b: BYTE) : DWORD :=
-  if ix == #0 then updateSlice 0 8 _ v b else
-  if ix == #1 then updateSlice 8 8 _ v b else
-  if ix == #2 then updateSlice 16 8 _ v b else
-  updateSlice 24 8 _ v b.
-  
   
 (* @TODO: update lemmas *)
