src/spredtotal.v
@@ -28,11 +28,6 @@ Proof. move => f x. destruct f; destruct x => //.  Qed.
 
 Require Import Coq.Logic.FunctionalExtensionality x86proved.charge.csetoid.
 
-Corollary sliceEqSome n1 n2 n3 (p q: BITS (n1+n2+n3)) : 
-  Some (slice n1 n2 n3 p) = Some (slice n1 n2 n3 q) ->
-  (forall i, n1 <= i < n1+n2 -> getBit p i = getBit q i).
-Proof. move => [H]. by apply sliceEq. Qed. 
-
 Lemma toPState_inj s1 s2 : toPState s1 === toPState s2 -> s1 = s2.
 Proof. move => H.
 destruct s1 as [s1r s1f s1m].
@@ -45,24 +40,7 @@ have H1 := H Registers (AnyRegPiece x #1).
 have H2 := H Registers (AnyRegPiece x #2).
 have H3 := H Registers (AnyRegPiece x #3).
 clear H.
-rewrite /getRegPiece eq_refl in H0. 
-rewrite /getRegPiece eq_refl in H1. replace (#1 == #0) with false in H1 by done. 
-rewrite /getRegPiece eq_refl in H2. 
-replace (#2 == #1) with false in H2 by done. replace (#2 == #0) with false in H2 by done. 
-rewrite /getRegPiece in H3. 
-replace (#3 == #0) with false in H3 by done. 
-replace (#3 == #1) with false in H3 by done. 
-replace (#3 == #2) with false in H3 by done.
-have S0 := sliceEqSome H0. 
-have S1 := sliceEqSome H1. 
-have S2 := sliceEqSome H2. 
-have S3 := sliceEqSome H3.
-apply allBitsEq. 
-move => i LT. 
-case LT8: (i < n8). apply (S0 _ LT8). 
-case LT16: (i < n16). apply S1. by rewrite LT16 leqNgt LT8. 
-case LT24: (i < n24). apply S2. by rewrite LT24 leqNgt LT16. 
-apply S3. by rewrite LT leqNgt LT24. 
+apply getRegPiece_ext; congruence.
 
 have E2: s1f = s2f.
 extensionality x. specialize (H Flags x). by injection H.
